Reorganise SystemF proof

proof/SystemF/Exp.v
@@ -1,54 +1,8 @@
 
+Require Export TyEnv.
+Require Export Ty.
+Require Export Ki.
 Require Export Env.
-Require Import Base.
-
-(* Kinds ************************************************************)
-Inductive ki : Type :=
- | KStar   : ki.
-
-Definition kienv := env ki.
-Hint Unfold kienv.
-
-
-(** Types ***********************************************************)
-Inductive ty  : Type :=
- | TCon    : nat -> ty
- | TVar    : nat -> ty
- | TForall : ty  -> ty
- | TFun    : ty  -> ty -> ty.
-Hint Constructors ty.
-
-Definition tyenv := env ty.
-Hint Unfold tyenv.
-
-
-(* Lift type indices that are at least a certain depth. *)
-Fixpoint liftTT (d: nat) (tt: ty) : ty :=
-  match tt with
-  | TCon _     => tt
-
-  |  TVar ix
-  => if le_gt_dec d ix
-      then TVar (S ix)
-      else tt
-
-  |  TForall t 
-  => TForall (liftTT (S d) t)
-
-  |  TFun t1 t2
-  => TFun    (liftTT d t1) (liftTT d t2)
-  end.
-Hint Unfold liftTT.
-
-(* Lift type indices in type environments. *)
-Definition liftTE d te    := map (liftTT d) te.
-Hint Unfold liftTE.
-
-Ltac lift_cases 
- := match goal with 
-     |  [ |- context [le_gt_dec ?n ?n'] ]
-     => case (le_gt_dec n n')
-    end.
 
 
 (** Expressions *****************************************************)
@@ -59,6 +13,58 @@ Inductive exp : Type :=
  | XLam  : ty  -> exp -> exp
  | XApp  : exp -> exp -> exp.
 Hint Constructors exp.
+
+
+(* Well Formedness **************************************************)
+(* A well formed expression is closed under the given environments *)
+Fixpoint wfX (ke: kienv) (te: tyenv) (xx: exp) : Prop := 
+ match xx with 
+ | XVar i     => exists t, get te i = Some t
+ | XLAM x     => wfX (ke :> KStar) (liftTE 0 te) x
+ | XAPP x t   => wfX ke te x  /\ wfT ke t
+ | XLam t x   => wfT ke t     /\ wfX ke (te :> t) x
+ | XApp x1 x2 => wfX ke te x1 /\ wfX ke te x2
+ end.
+Hint Unfold wfX.
+
+
+(* Closed expressions are well formed under empty environments *)
+Definition closedX (xx: exp) : Prop
+ := wfX Empty Empty xx.
+Hint Unfold closedX.
+
+
+(* Values are closed expressions that cannot be reduced further *)
+Inductive value : exp -> Prop :=
+ | Value_lam 
+   : forall t x
+   , closedX (XLam t x) -> value (XLam t x)
+
+ | Value_LAM
+   : forall x
+   , closedX (XLAM x)   -> value (XLAM x).
+
+Hint Constructors value.
+
+
+(* Lifting **********************************************************)
+(* Lift type indices that are at least a certain depth. *)
+Fixpoint liftTX (d: nat) (xx: exp) : exp :=
+  match xx with
+  |  XVar _     => xx
+
+  |  XLAM x     
+  => XLAM (liftTX (S d) x)
+
+  |  XAPP x t 
+  => XAPP (liftTX d x)  (liftTT d t)
+ 
+  |  XLam t x   
+  => XLam (liftTT d t)  (liftTX d x)
+
+  |  XApp x1 x2
+  => XApp (liftTX d x1) (liftTX d x2)
+ end.
 
 
 (* Lift value indices in expressions.
@@ -82,5 +88,51 @@ Fixpoint liftXX (d: nat) (xx: exp) : exp :=
   |  XApp x1 x2
   => XApp (liftXX d x1) (liftXX d x2)
  end.
+
+
+(* Substitution *****************************************************)
+(* Substitution of Types in Exps *)
+Fixpoint substTX (d: nat) (u: ty) (xx: exp) : exp :=
+  match xx with
+  | XVar _     => xx
+
+  |  XLAM x     
+  => XLAM (substTX (S d) (liftTT 0 u) x)
+
+  |  XAPP x t
+  => XAPP (substTX d u x)  (substTT d u t)
+
+  |  XLam t x
+  => XLam (substTT d u t)  (substTX d u x)
+
+  |  XApp x1 x2
+  => XApp (substTX d u x1) (substTX d u x2)
+ end.
+
+
+(* Substitution of Exps in Exps *)
+Fixpoint substXX (d: nat) (u: exp) (xx: exp) : exp :=
+  match xx with
+  | XVar ix    
+  => match nat_compare ix d with
+     | Eq => u
+     | Gt => XVar (ix - 1)
+     | _  => XVar  ix
+     end
+
+  |  XLAM x
+  => XLAM (substXX d (liftTX 0 u) x)
+
+  |  XAPP x t
+  => XAPP (substXX d u x) t
+
+  |  XLam t x
+  => XLam t (substXX (S d) (liftXX 0 u) x)
+
+  |  XApp x1 x2
+  => XApp (substXX d u x1) (substXX d u x2)
+  end.
+
+
 
 
