proof/SystemF/Ki.v
@@ -1,0 +1,13 @@
+
+Require Export Env.
+Require Export Base.
+
+
+(* Kinds ************************************************************)
+Inductive ki : Type :=
+ | KStar   : ki.
+
+Definition kienv := env ki.
+Hint Unfold kienv.
+
+
