proof/SystemF/Ty.v
@@ -1,0 +1,209 @@
+
+Require Export Ki.
+Require Export Env.
+Require Export Base.
+
+
+(* Types ************************************************************)
+Inductive ty  : Type :=
+ | TCon    : nat -> ty
+ | TVar    : nat -> ty
+ | TForall : ty  -> ty
+ | TFun    : ty  -> ty -> ty.
+Hint Constructors ty.
+
+
+(* Well Formedness **************************************************)
+(* Well formed types are closed under the given kind environment *)
+Fixpoint wfT (ke: kienv) (tt: ty) : Prop := 
+ match tt with
+ | TCon _     => True
+ | TVar i     => exists k, get ke i = Some k
+ | TForall t  => wfT (ke :> KStar) t
+ | TFun t1 t2 => wfT ke t1 /\ wfT ke t2
+ end.
+Hint Unfold wfT.
+
+
+(* Type is closed under an empty kind environment. *)
+Definition closedT (tt: ty) : Prop
+ := wfT Empty tt.
+Hint Unfold closedT.
+
+
+(* Lifting *********************************************************)
+(* Lift type indices that are at least a certain depth. *)
+Fixpoint liftTT (d: nat) (tt: ty) : ty :=
+  match tt with
+  | TCon _     => tt
+
+  |  TVar ix
+  => if le_gt_dec d ix
+      then TVar (S ix)
+      else tt
+
+  |  TForall t 
+  => TForall (liftTT (S d) t)
+
+  |  TFun t1 t2
+  => TFun    (liftTT d t1) (liftTT d t2)
+  end.
+Hint Unfold liftTT.
+
+
+(* Tactic to help deal with lifting functions *)
+Ltac lift_cases 
+ := match goal with 
+     |  [ |- context [le_gt_dec ?n ?n'] ]
+     => case (le_gt_dec n n')
+    end.
+
+
+(* Substitution *****************************************************)
+(* Substitution of Types in Types. *)
+Fixpoint substTT (d: nat) (u: ty) (tt: ty) : ty 
+ := match tt with
+    |  TCon _     
+    => tt
+ 
+    | TVar ix
+    => match nat_compare ix d with
+       | Eq => u
+       | Gt => TVar (ix - 1)
+       | _  => TVar  ix
+       end
+
+    |  TForall t  
+    => TForall (substTT (S d) (liftTT 0 u) t)
+
+    |  TFun t1 t2 
+    => TFun (substTT d u t1) (substTT d u t2)
+  end.
+
+
+(* Lemmas ***********************************************************)
+(* Changing the order of lifting. *)
+Lemma liftTT_liftTT
+ :  forall n n' t
+ ,  liftTT n              (liftTT (n + n') t) 
+ =  liftTT (1 + (n + n')) (liftTT n t).
+Proof.
+ intros. gen n n'.
+ induction t; intros; auto.
+
+ Case "TVar".
+  simpl.
+  repeat (unfold liftTT; lift_cases; intros); burn.
+
+ Case "TForall".
+  simpl.
+  assert (S (n + n') = (S n) + n'). omega. rewrite H. 
+  rewrite IHt. auto.
+
+ Case "TFun".
+  simpl. apply f_equal2; auto.
+Qed.  
+
+
+(* If we lift at depth d, this creates an empty space and
+   substituting into it doens't do anything. *)
+Lemma substTT_liftTT
+ :  forall d t1 t2
+ ,  substTT d t2 (liftTT d t1) = t1.
+Proof.
+ intros. gen d t2.
+ induction t1; intros; eauto.
+
+ Case "TVar".
+  simpl; lift_cases; unfold substTT;
+   fbreak_nat_compare; intros;
+   burn.
+
+ Case "TForall".
+  simpl. 
+  rewrite IHt1. auto.
+
+ Case "TFun".
+  simpl.
+  rewrite IHt1_1.
+  rewrite IHt1_2. auto.
+Qed.
+
+
+(* Lifting after substitution *)
+Lemma liftTT_substTT
+ :  forall n n' t1 t2
+ ,  liftTT n (substTT (n + n') t2 t1)
+ =  substTT (1 + n + n') (liftTT n t2) (liftTT n t1).
+Proof.
+ intros. gen n n' t2.
+ induction t1; intros; eauto.
+
+ Case "TVar".
+  repeat (simpl; fbreak_nat_compare; 
+          try lift_cases; try intros);
+   burn.
+
+ Case "TForall".
+  simpl.
+  rewrite (IHt1 (S n) n'). simpl.
+  rewrite (liftTT_liftTT 0 n). auto.
+
+ Case "TFun".
+  simpl.
+  rewrite IHt1_1. auto.
+  rewrite IHt1_2. auto.
+Qed.
+
+
+Lemma liftTT_substTT'
+ :  forall n n' t1 t2
+ ,  liftTT (n + n') (substTT n t2 t1)
+ =  substTT n (liftTT (n + n') t2) (liftTT (1 + n + n') t1).
+Proof.
+ intros. gen n n' t2.
+ induction t1; intros; auto.
+
+ Case "TVar".
+  repeat ( unfold liftTT; unfold substTT; fold liftTT; fold substTT
+         ; try lift_cases; try fbreak_nat_compare
+         ; intros); burn.
+
+ Case "TForall".
+  simpl. f_equal.
+  rewrite (IHt1 (S n) n'). f_equal.
+   simpl. rewrite (liftTT_liftTT 0 (n + n')). auto.
+
+ Case "TFun".
+  simpl. f_equal.
+   apply IHt1_1.
+   apply IHt1_2.
+Qed.
+
+
+(* Commuting substitutions. *)
+Lemma substTT_substTT
+ :  forall n m t1 t2 t3
+ ,  substTT (n + m) t3 (substTT n t2 t1)
+ =  substTT n (substTT (n + m) t3 t2)
+              (substTT (1 + n + m) (liftTT n t3) t1).
+Proof.
+ intros. gen n m t2 t3.
+ induction t1; intros; auto.
+
+ Case "TVar".
+  repeat (simpl; fbreak_nat_compare; burn).
+  rewrite substTT_liftTT. auto.
+
+ Case "TForall".
+  simpl. f_equal.
+  rewrite (IHt1 (S n) m). f_equal.
+   simpl. rewrite (liftTT_substTT 0 (n + m)). auto.
+   simpl. rewrite (liftTT_liftTT 0 n). auto.  
+
+ Case "TFun".
+  simpl. f_equal.
+   apply IHt1_1.
+   apply IHt1_2.
+Qed.
+
